@prefix :        <EnvironmentalFactors/> .
@prefix externalfactors:  <http://www.purl.org/oema/externalfactors/> .
@prefix owl:     <http://www.w3.org/2002/07/owl#> .
@prefix ns:      <http://creativecommons.org/ns#> .
@prefix xsd:     <http://www.w3.org/2001/XMLSchema#> .
@prefix swrlb:   <http://www.w3.org/2003/11/swrlb#> .
@prefix swrl:    <http://www.w3.org/2003/11/swrl#> .
@prefix skos:    <http://www.w3.org/2004/02/skos/core#> .
@prefix rdfs:    <http://www.w3.org/2000/01/rdf-schema#> .
@prefix rdf:     <http://www.w3.org/1999/02/22-rdf-syntax-ns#> .
@prefix terms:   <http://purl.org/dc/terms/> .
@prefix swrlx:   <http://www.w3.org/2003/11/swrlx#> .
@prefix owl2:    <http://www.w3.org/2006/12/owl2#> .
@prefix time:    <http://www.w3.org/2006/time#> .
@prefix WeatherOntology:  <https://www.auto.tuwien.ac.at/downloads/thinkhome/ontology/WeatherOntology.owl#> .
@prefix dc:      <http://purl.org/dc/elements/1.1/> .

externalfactors:ExternalFactor
      a       owl:Class .

ns:license
      a       owl:AnnotationProperty .

time:Instant
      a       owl:Class .

externalfactors:EnvironmentalFactor
      a       owl:Class ;
      rdfs:comment "This class represents environmental factors, which refer to the principal air pollutants in the urban area (e.g. total suspended particulate matter, sul-phur dioxide, nitrogen dioxide, carbon monoxide, ozone, lead, etc.)."@en ;
      rdfs:label "EnvironmentalFactor"@en ;
      rdfs:subClassOf externalfactors:ExternalFactor ;
      rdfs:subClassOf
              [ a       owl:Restriction ;
                owl:onClass
                        [ a       owl:Class ;
                          owl:unionOf (time:Instant time:Interval)
                        ] ;
                owl:onProperty WeatherOntology:hasObservationTime ;
                owl:qualifiedCardinality
                        "1"^^xsd:nonNegativeInteger
              ] .

<http://www.purl.org/dabgeo/common-domain/environmentalfactors>
      a       owl:Ontology ;
      rdfs:comment """The 'Environmental Factors' ontology module represents different environmental factors that affect energy performance such as air pollutants or weahter related environmental factors, i.e., luminity. 
This ontology module reuses the knowledge of the 'External Factors' ontology module, as well as the 'Time' external ontology.

Information about changes compared to version 1.1
*********************************************************
We have changed the names of ontology layers and documented missing classes."""@en ;
      ns:license "https://creativecommons.org/licenses/by-nc/4.0/" ;
      dc:creator "Javier Cuenca <mailto:jcuenca@mondragon.edu>"@en ;
      dc:title "Environmental Factors ontology"@en ;
      terms:issued "2018-02-09"@en ;
      terms:modified "2019-02-22"@en ;
      owl:imports <http://www.w3.org/2006/time#2016> , <http://www.purl.org/dabgeo/common-domain/externalfactors> ;
      owl:versionInfo "2.0"@en .

WeatherOntology:hasObservationTime
      a       owl:ObjectProperty ;
      rdfs:comment "This property relates an energy parameter with the period of time when it is measured." ;
      rdfs:label "hasObservationTime"@en ;
      rdfs:range
              [ a       owl:Class ;
                owl:unionOf (time:Instant time:Interval)
              ] .

time:Interval
      a       owl:Class .
